CertiGC/verif_resume.v
@@ -3,11 +3,12 @@ Require Import RamifyCoq.CertiGC.gc_spec.
 Lemma body_resume: semax_body Vprog Gprog f_resume resume_spec.
 Proof.
   start_function.
-  remember (glabel g) as tinfo. unfold thread_info_rep.
-  destruct (EquivDec.equiv_dec (ti_heap_p tinfo) nullval).
-  1: hnf in e; exfalso; tauto. clear c. Intros. unfold heap_struct_rep. forward.
+  unfold thread_info_rep. destruct (Val.eq (ti_heap_p t_info) nullval).
+  1: hnf in e; exfalso; tauto. clear n. Intros. unfold heap_struct_rep. forward. 
   unfold fun_info_rep. forward. 1: entailer!. rewrite Znth_0_cons.
-  forward_if True; [forward; entailer!|exfalso; destruct tinfo; simpl in *; tauto|].
-  Intros. remember (ti_heap_p tinfo) as h. remember (ti_heap tinfo) as theap.
-  
+  forward_if True; [forward; entailer!|exfalso; destruct t_info; simpl in *; tauto|].
+  Intros. remember (ti_heap_p t_info) as h. remember (ti_heap t_info) as theap.
+  pose proof (sound_gg g). simpl in H1.
+  forward; rewrite Znth_0_cons.
+  - entailer!.
 Abort.
